Pseudo Datalog solver implemented

Pseudo_Datalog.thy
@@ -1,7 +1,9 @@
 theory Pseudo_Datalog
   imports PDDL_Sema_Supplement Normalization_Definitions
-    Formula_Utils
+    Formula_Utils Graph_Funs String_Shenanigans
 begin
+
+term nat_upto
 
 text \<open>
 Here, reachability analysis is performed directly on the PDDL problem data structure, instead of
@@ -15,20 +17,15 @@ The input problem is assumed to be:
     TODO: re-evaluate if the structure of the goal really matters here...
 \<close>
 
-term Action_Schema
-(* (name: name)
-  (parameters: "(variable \<times> type) list")
-  (precondition: "term atom formula")
-  (effect: "term ast_effect") *)
-
-term ast_domain.instantiate_action_schema
+type_synonym fact_orga = "predicate \<Rightarrow> object list list"
+type_synonym partial_args = "variable \<rightharpoonup> object"
 
 datatype action_clause = AClause
-  (name: name)
-  (parameters: "(variable \<times> type) list")
-  (pred_pre: "term atom formula list")
-  (cond_pre: "term atom formula list")
-  (pos: "term atom formula list")
+  (cl_name: name)
+  (cl_params: "(variable \<times> type) list")
+  (cl_pred_pre: "term atom formula list")
+  (cl_cond_pre: "term atom formula list")
+  (cl_pos: "term atom formula list")
 
 definition pos_lits_of :: "'a atom formula \<Rightarrow> 'a atom formula list" where
   "pos_lits_of F = filter is_predAtom (un_and F)"
@@ -36,20 +33,261 @@ definition cond_lits_of :: "'a atom formula \<Rightarrow> 'a atom formula list" 
   "cond_lits_of F = filter (HOL.Not \<circ> is_predAtom) (un_and F)"
 
 
-  
-
-
-
+(* TODO: add action predicate to a? *)
 fun as_action_clause :: "ast_action_schema \<Rightarrow> action_clause" where
   "as_action_clause (Action_Schema n params pre (Effect a d)) =
-    AClause n params (filter is_predAtom (un_and pre)) [] a"
+    AClause n params (pos_lits_of pre) (cond_lits_of pre) a"
 
+(* fact_orga functionality *)
+fun update_facts :: "object atom formula list \<Rightarrow> fact_orga \<Rightarrow> fact_orga" where
+  "update_facts [] orga = orga" |
+  "update_facts (Atom (predAtm p args) # fs) orga =
+    (let orga' = update_facts fs orga in
+    orga'(p := args # orga' p))" |
+  "update_facts (_ # fs) orga = undefined" (* not pred atom *)
+abbreviation organize_facts :: "object atom formula list \<Rightarrow> fact_orga" where
+  "organize_facts fs \<equiv> update_facts fs (\<lambda>p. [])"
+fun in_orga :: "object atom formula \<Rightarrow> fact_orga \<Rightarrow> bool" where
+  "in_orga (Atom (predAtm p args)) orga \<longleftrightarrow> args \<in> set (orga p)" |
+  "in_orga _ orga \<longleftrightarrow> undefined" (* not pred atom *)
+definition (in ast_problem) enumerate_orga :: "fact_orga \<Rightarrow> object atom formula list" where
+  "enumerate_orga facts = [Atom (predAtm (pred p) args). p \<leftarrow> predicates D, args \<leftarrow> facts (pred p)]"
 
+(* partial_args functionality *)
+fun fix_to :: "object list \<Rightarrow> term list \<Rightarrow> partial_args \<Rightarrow> partial_args option" where
+  "fix_to [] [] args = Some args" |
+  "fix_to (obj # objs) (term.CONST x # ts) args = (if obj = x then fix_to objs ts args else None)" |
+  "fix_to (obj # objs) (term.VAR x # ts) args = (case args x of
+    None \<Rightarrow> fix_to objs ts (args(x \<mapsto> obj)) |
+    Some y \<Rightarrow> (if y = obj then fix_to objs ts args else None))" |
+  "fix_to _ _ args = undefined" (* different lengths *)
 
+abbreviation fix_to' :: "object list \<Rightarrow> term atom formula \<Rightarrow> partial_args \<Rightarrow> partial_args option" where
+  "fix_to' f c args \<equiv> fix_to f (atom.arguments (un_Atom c)) args"
+abbreviation as_arg_list :: "(variable \<times> type) list \<Rightarrow> partial_args \<Rightarrow> object option list" where
+  "as_arg_list vs args \<equiv> map (args \<circ> fst) vs"
+
+(* instantiating action clauses *)
+abbreviation "satisfies_cond params args c \<equiv>
+  valuation {} \<Turnstile> map_atom_fmla (ac_tsubst params args) c"
+abbreviation satisfies_conds where
+  "satisfies_conds params conds args \<equiv>
+    list_all (satisfies_cond params args) conds"
+fun finish_args :: "'a option list \<Rightarrow> 'a list \<Rightarrow> 'a list" where
+  "finish_args [] [] = []" |
+  "finish_args (None # partial) (y # ys) = y # finish_args partial ys" |
+  "finish_args (Some x # partial) ys = x # finish_args partial ys" |
+  "finish_args _ _ = undefined" (* number of Nones does not match length of ys *)
+  (* other cases for length ys \<noteq> count None xs *)
+fun consequence_of where "consequence_of (AClause n params preds cond add) args =
+  map (map_atom_fmla (ac_tsubst params args)) add"
 
 context ast_problem begin
+
+definition "a_clauses \<equiv> map as_action_clause (actions D)"
+definition "pred_clauses \<equiv> filter (\<lambda>c. cl_pred_pre c \<noteq> []) a_clauses"
+definition "fact_clauses \<equiv> filter (\<lambda>c. cl_pred_pre c = []) a_clauses"
+abbreviation "const_names \<equiv> map fst all_consts"
+
+(* set of initial facts, considering some clauses may have an empty body... *)
+(* all possible parameterizations for a fact *)
+(* corresponds to level 6 *)
+fun all_fact_paramz :: "action_clause \<Rightarrow> object list list" where
+  "all_fact_paramz (AClause n params preds cond add) =
+    all_combos (satisfies_conds params cond) (replicate (length params) const_names)"
+abbreviation all_fact_consqs where
+  "all_fact_consqs r \<equiv> concat (map (consequence_of r) (all_fact_paramz r))"
+definition "pseudo_init \<equiv> concat (map all_fact_consqs fact_clauses)"
+definition "init' \<equiv> conc_unique pseudo_init (init P)"
+
+(* Level 6: fix list of optional args, for every satisfied finished parameterization...*)
+fun all_finished_paramz :: "action_clause \<Rightarrow> object option list \<Rightarrow> object list list" where
+  "all_finished_paramz (AClause n params preds cond add) partial =
+    all_combos (satisfies_conds params cond \<circ> finish_args partial)
+      (replicate (count_list partial None) const_names)"
+
+(* Level 5: fix w r i j, for f \<in> facts, where f matches r!j...
+  (the f chosen from 'previous' j is a fixed parameter in the recursion. Initially, it's w.)
+  (i is 'integrated' into args, j is the recursive parameter)*)
+fun all_insts_owa_aux
+  :: "fact_orga \<Rightarrow> object list \<Rightarrow> partial_args \<Rightarrow> term atom formula list
+    \<Rightarrow> partial_args list"
+  where
+  "all_insts_owa_aux facts f args [] = undefined" | (* should not be called on empty clauses *)
+  "all_insts_owa_aux facts f args [c] = (case fix_to' f c args of
+    Some a \<Rightarrow> [a] | None \<Rightarrow> [])" |
+  "all_insts_owa_aux facts f args (c#c'#cs) = (case fix_to' f c args of Some a' \<Rightarrow>
+    concat [all_insts_owa_aux facts f' a' (c'#cs). f' \<leftarrow> facts (unPredAtom c')] | None \<Rightarrow> [])"
+
+definition to_front :: "'a list \<Rightarrow> nat \<Rightarrow> 'a list" where
+  "to_front xs i = (xs ! i) # (take i xs @ drop (i + 1) xs)"
+
+(* Level 4: fix w r i, IF r!i matches w THEN for all j...
+  Two checks can fail here: Either the predicate symbols of r!i and w don't match.
+  Or their parameters can't be unified, i.e. when w=P(a,b) and r!i=P(x,x) *)
+fun all_insts_of_with_at'' :: "object atom formula \<Rightarrow> fact_orga \<Rightarrow> action_clause \<Rightarrow> nat \<Rightarrow> partial_args list" where
+  "all_insts_of_with_at'' f facts c i =
+    
+    (let preds = cl_pred_pre c in
+      (if unPredAtom f \<noteq> unPredAtom (preds ! i) then [] else let
+         f_objs = atom.arguments (un_Atom f) in
+      case fix_to' f_objs (preds ! i) (\<lambda>x. None) of
+        Some args\<^sub>0 \<Rightarrow> all_insts_owa_aux facts f_objs args\<^sub>0 (to_front preds i) |
+        None \<Rightarrow> []))"
+
+(* Level 4: fix w r, transform partial args into list of optional *)
+fun all_insts_of_with_at' :: "object atom formula \<Rightarrow> fact_orga \<Rightarrow> action_clause \<Rightarrow> nat \<Rightarrow> object option list list" where
+  "all_insts_of_with_at' f facts c i =
+    (let partials = all_insts_of_with_at'' f facts c i in
+    map (as_arg_list (cl_params c)) partials)"
+
+(* Level 4: fix w r, given partial args, obtain finished args *)
+fun all_insts_of_with_at :: "object atom formula \<Rightarrow> fact_orga \<Rightarrow> action_clause \<Rightarrow> nat \<Rightarrow> object list list" where
+  "all_insts_of_with_at f facts c i =
+    (let partials = all_insts_of_with_at' f facts c i in
+    [finish_args p extra. p \<leftarrow> partials, extra \<leftarrow> all_finished_paramz c p])"
+
+(* Level 3: fix w r, for i in range(body(r))... *)
+fun all_insts_of_with :: "object atom formula \<Rightarrow> fact_orga \<Rightarrow> action_clause \<Rightarrow> object list list" where
+  "all_insts_of_with f facts c = concat (map (all_insts_of_with_at f facts c) (nat_range (length (cl_pred_pre c))))"
+
+(* Level 3: fix w r, given args, apply heads *)
+fun all_derivs_of :: "object atom formula \<Rightarrow> fact_orga \<Rightarrow> action_clause \<Rightarrow> object atom formula list" where
+  "all_derivs_of f facts c = [a. args \<leftarrow> all_insts_of_with f facts c, a \<leftarrow> consequence_of c args]"
+
+(* Level 2: fix w, for r in pred_clauses... *)
+fun all_derivs where
+  "all_derivs f facts = concat (map (all_derivs_of f facts) pred_clauses)"
+
+(* Level 1: for w in working set... *)
+function (sequential) semi_naive_aux where
+  "semi_naive_aux [] facts = facts" |
+  "semi_naive_aux (w#works) facts =
+    (let derivs = all_derivs w facts;
+         news = filter (\<lambda>x. \<not> in_orga x facts) derivs;
+         facts' = update_facts news facts in
+    semi_naive_aux (works @ news) facts')"
+  by (pat_completeness) blast+
+termination semi_naive_aux proof
+  show "wf undefined" sorry
+  show "\<And>w works facts x xa xb.
+       x = all_derivs w facts \<Longrightarrow>
+       xa = filter (\<lambda>x. \<not> in_orga x facts) x \<Longrightarrow>
+       xb = update_facts xa facts \<Longrightarrow> ((works @ xa, xb), w # works, facts) \<in> undefined"
+    sorry
+qed
+
+definition "semi_naive_eval \<equiv> (\<lambda>x. semi_naive_aux x (organize_facts x)) init'"
+
 end
 
+lemmas pseudo_datalog_code =
+  ast_domain.subst_term.simps (* TODO move*)
+  ast_problem.enumerate_orga_def
+  ast_problem.a_clauses_def
+  ast_problem.pred_clauses_def
+  ast_problem.fact_clauses_def
+  ast_problem.all_fact_paramz.simps
+  ast_problem.pseudo_init_def
+  ast_problem.init'_def
+  ast_problem.all_finished_paramz.simps
+  ast_problem.all_insts_owa_aux.simps
+  ast_problem.all_insts_of_with_at''.simps
+  ast_problem.all_insts_of_with_at'.simps
+  ast_problem.all_insts_of_with_at.simps
+  ast_problem.all_insts_of_with.simps
+  ast_problem.all_derivs_of.simps
+  ast_problem.all_derivs.simps
+  ast_problem.semi_naive_aux.simps
+  ast_problem.semi_naive_eval_def
+
+declare pseudo_datalog_code[code]
+
+abbreviation "as_atom n args \<equiv> Atom (predAtm (Pred n) args)"
+abbreviation "var n \<equiv> term.VAR (Var n)"
+abbreviation "cst n \<equiv> term.CONST (Obj n)"
+
+definition "action_move \<equiv> Action_Schema
+      ''move''
+      [(Var ''what'', \<omega>), (Var ''from'', \<omega>), (Var ''to'', \<omega>)]
+      (as_atom ''at'' [term.VAR (Var ''what''), term.VAR (Var ''from'')] \<^bold>\<and>
+        as_atom ''path'' [term.VAR (Var ''from''), term.VAR (Var ''to'')])
+      (Effect [as_atom ''at'' [var ''what'', var ''to'']]
+              [as_atom ''at'' [var ''what'', var ''from'']])"
+definition "action_DE \<equiv> Action_Schema
+      ''DE''
+      [(Var ''d'', \<omega>), (Var ''e'', \<omega>), (Var ''x'', \<omega>)]
+      (Atom (Eq (var ''d'') (cst ''D'')) \<^bold>\<and> Atom (Eq (var ''e'') (cst ''E'')))
+      (Effect [as_atom ''path'' [var ''d'', var ''e'']] [])"
+definition "action_omni \<equiv> Action_Schema
+      ''omni''
+      [(Var ''where'', \<omega>)]
+      (\<^bold>\<not>(Atom (Eq (var ''where'') (cst ''w''))) \<^bold>\<and>
+      (\<^bold>\<not>(Atom (Eq (var ''where'') (cst ''x''))) \<^bold>\<and>
+      (\<^bold>\<not>(Atom (Eq (var ''where'') (cst ''B''))) \<^bold>\<and>
+       \<^bold>\<not>(Atom (Eq (var ''where'') (cst ''y''))))))
+      (Effect [as_atom ''at'' [cst ''w'', var ''where'']] [])"
+definition "action_foo \<equiv> Action_Schema
+      ''foo''
+      [(Var ''a'', \<omega>), (Var ''b'', \<omega>)]
+      (Atom (Eq (var ''a'') (var ''b'')) \<^bold>\<and>
+      (as_atom ''at'' [cst ''x'', var ''a'']))
+      (Effect [as_atom ''foo'' [var ''a'', var ''b'']] [])"
+
+definition my_prob ("\<Pi>") where "my_prob \<equiv> Problem
+  (Domain
+    []
+    [PredDecl (Pred ''at'') [\<omega>, \<omega>],
+     PredDecl (Pred ''path'') [\<omega>, \<omega>],
+     PredDecl (Pred ''foo'') [\<omega>, \<omega>]]
+    []
+    [action_DE, action_omni, action_move, action_foo])
+  [(Obj ''A'', \<omega>), (Obj ''B'', \<omega>), (Obj ''C'', \<omega>), (Obj ''D'', \<omega>), (Obj ''E'', \<omega>),
+   (Obj ''x'', \<omega>), (Obj ''y'', \<omega>), (Obj ''w'', \<omega>)]
+  [as_atom ''at'' [Obj ''x'', Obj ''A''], as_atom ''at'' [Obj ''y'', Obj ''D''],
+   as_atom ''path'' [Obj ''A'', Obj ''B''], as_atom ''path'' [Obj ''B'', Obj ''C''],
+   as_atom ''path'' [Obj ''C'', Obj ''A''], as_atom ''at'' [Obj ''w'', Obj ''A'']]
+  \<bottom>"
+
+interpretation Pi: ast_problem \<Pi> done
+
+value "Pi.all_finished_paramz (as_action_clause action_foo) [Some (Obj ''A''), None]"
+
+
+value "Pi.pred_clauses"
+value "Pi.fact_clauses"
+value "Pi.enumerate_orga (organize_facts Pi.init')"
+
+abbreviation (input) "facto \<equiv> (as_atom ''path'' [Obj ''A'', Obj ''B''])"
+abbreviation "orga0 \<equiv> organize_facts Pi.init'"
+abbreviation "clause \<equiv> as_action_clause action_move"
+
+thm Pi.all_insts_of_with_at''.simps[of facto orga0 clause 0]
+thm Pi.all_insts_owa_aux.simps
+value "cl_pred_pre clause"
+abbreviation "args0 \<equiv> fix_to' (atom.arguments (un_Atom facto)) ((cl_pred_pre clause) ! 0) (\<lambda>x. None)"
+value "as_arg_list (cl_params clause) (the args0)"
+value "Pi.all_insts_owa_aux
+  orga0
+  (atom.arguments (un_Atom facto))
+  (the args0)
+  (cl_pred_pre clause)"
+value "fix_to' (atom.arguments (un_Atom facto)) ((cl_pred_pre clause) ! 0) (the args0)"
+
+value "Pi.all_insts_of_with_at'' facto (organize_facts Pi.init') (as_action_clause action_move) 1"
+value "Pi.all_insts_of_with_at' facto (organize_facts Pi.init') (as_action_clause action_move) 0"
+value "Pi.all_insts_of_with_at facto (organize_facts Pi.init') (as_action_clause action_move) 0"
+value "consequence_of (as_action_clause action_move) [Obj ''A'', Obj ''B'', Obj ''C'']"
+value "Pi.all_insts_of_with facto (organize_facts Pi.init') (as_action_clause action_move)"
+value "Pi.all_derivs_of facto (organize_facts Pi.init') (as_action_clause action_move)"
+value "Pi.all_derivs facto (organize_facts Pi.init')"
+value "Pi.enumerate_orga orga0"
+value "Pi.enumerate_orga (update_facts (Pi.all_derivs facto (organize_facts Pi.init'))orga0)"
+value "Pi.enumerate_orga (Pi.semi_naive_eval)"
+
+abbreviation "d1 \<equiv> Pi.all_derivs (as_atom ''path'' [Obj ''A'', Obj ''B'']) orga0"
+value d1
+value "Pi.enumerate_orga (update_facts d1 orga0)"
 
 subsection \<open> Proofs \<close>
 
@@ -61,6 +299,7 @@ lemma "set (un_and xs) = set (pos_lits_of xs) \<union> set (cond_lits_of xs)"
 
 context wf_relaxed_normed_prob begin
 end
+
 
 
 end
